src/Narcissus/Examples/NetworkStack/IPv4Header.v
@@ -32,43 +32,43 @@ Open Scope Tuple_scope.
 (* Our source data type for IP packets. *)
 Definition IPv4_Packet :=
   @Tuple <"TotalLength" :: word 16,
-          "ID" :: word 16,
-          "DF" :: bool, (* Don't fragment flag *)
-          "MF" :: bool, (*  Multiple fragments flag *)
-          "FragmentOffset" :: word 13,
-          "TTL" :: word 8,
-          "Protocol" :: EnumType ["ICMP"; "TCP"; "UDP"],
-          "SourceAddress" :: word 32,
-          "DestAddress" :: word 32,
-          "Options" :: list (word 32)>.
+  "ID" :: word 16,
+  "DF" :: bool, (* Don't fragment flag *)
+  "MF" :: bool, (*  Multiple fragments flag *)
+  "FragmentOffset" :: word 13,
+  "TTL" :: word 8,
+  "Protocol" :: EnumType ["ICMP"; "TCP"; "UDP"],
+  "SourceAddress" :: word 32,
+  "DestAddress" :: word 32,
+  "Options" :: list (word 32)>.
 
 (* Protocol Numbers from [RFC5237]*)
 Definition ProtocolTypeCodes : Vector.t (word 8) 3 :=
   [WO~0~0~0~0~0~0~0~1; (* ICMP: 1*)
-   WO~0~0~0~0~0~1~1~0; (* TCP:  6*)
-   WO~0~0~0~1~0~0~0~1  (* UDP:  17*)
+     WO~0~0~0~0~0~1~1~0; (* TCP:  6*)
+     WO~0~0~0~1~0~0~0~1  (* UDP:  17*)
   ].
 
 Definition IPv4_Packet_Header_Len (ip4 : IPv4_Packet) := 5 + |ip4!"Options"|.
 
 Definition IPv4_Packet_Format (ip4 : IPv4_Packet)  :=
-          (format_word (natToWord 4 4)
-    ThenC format_nat 4 (IPv4_Packet_Header_Len ip4)
-    ThenC format_unused_word 8 (* TOS Field! *)
-    ThenC format_word ip4!"TotalLength"
-    ThenC format_word ip4!"ID"
-    ThenC format_unused_word 1 (* Unused flag! *)
-    ThenC format_bool ip4!"DF"
-    ThenC format_bool ip4!"MF"
-    ThenC format_word ip4!"FragmentOffset"
-    ThenC format_word ip4!"TTL"
-    ThenC format_enum ProtocolTypeCodes ip4!"Protocol"
-    DoneC)
+  (format_word (natToWord 4 4)
+               ThenC format_nat 4 (IPv4_Packet_Header_Len ip4)
+               ThenC format_unused_word 8 (* TOS Field! *)
+               ThenC format_word ip4!"TotalLength"
+               ThenC format_word ip4!"ID"
+               ThenC format_unused_word 1 (* Unused flag! *)
+               ThenC format_bool ip4!"DF"
+               ThenC format_bool ip4!"MF"
+               ThenC format_word ip4!"FragmentOffset"
+               ThenC format_word ip4!"TTL"
+               ThenC format_enum ProtocolTypeCodes ip4!"Protocol"
+               DoneC)
     ThenChecksum IPChecksum_Valid' OfSize 16
     ThenCarryOn (format_word ip4!"SourceAddress"
-    ThenC format_word ip4!"DestAddress"
-    ThenC format_list format_word ip4!"Options"
-    DoneC)%format.
+                             ThenC format_word ip4!"DestAddress"
+                             ThenC format_list format_word ip4!"Options"
+                             DoneC)%format.
 
 Definition IPv4_Packet_OK (ipv4 : IPv4_Packet) :=
   lt (|ipv4!"Options"|) 11 /\
@@ -87,30 +87,6 @@ Defined.
 Definition ipv4_encoder_impl r {sz} v :=
   Eval simpl in (projT1 ipv4_encoder r sz v 0 tt).
 
-Definition IPv4_Packet_formatd_measure (ipv4_b : ByteString)
-  : nat :=
-  match (`(u, b') <- decode_unused_word' 4 ipv4_b;
-           decode_word' 4 b') with
-  | Some n => 32 * wordToNat (fst n)
-  | None => 0
-  end.
-
-Lemma IPv4_Packet_Headiner_Len_Bound
-  : forall (a : IPv4_Packet) (a_OK : IPv4_Packet_OK a),
-    BinNat.N.lt (BinNat.N.of_nat (IPv4_Packet_Header_Len a)) (Npow2 4).
-Proof.
-  unfold IPv4_Packet_Header_Len.
-  intros; unfold IPv4_Packet_OK in a_OK.
-  destruct a_OK.
-  rewrite <- BinNat.N.compare_lt_iff.
-  rewrite Nnat.N2Nat.inj_compare.
-  rewrite Nnat.Nat2N.id.
-  rewrite <- Compare_dec.nat_compare_lt.
-  simpl.
-  unfold BinPos.Pos.to_nat; simpl.
-  auto with arith.
-Qed.
-
 Lemma IPv4_Packet_Header_Len_eq
   : forall data len,
     IPv4_Packet_Header_Len data = len
@@ -121,400 +97,16 @@ Proof.
   rewrite H; reflexivity.
 Qed.
 
-Lemma computes_to_compose_decode_unused_word
-  : forall (sz : nat) (w : word sz) (ctx ctx'' : CacheFormat)
-           (rest : CacheFormat -> Comp (ByteString * CacheFormat))
-           (b : ByteString),
-    (format_word w ThenC rest) ctx ↝ (b, ctx'') ->
-    exists (b' : ByteString) (ctx' : CacheFormat),
-      rest ctx' ↝ (b', ctx'') /\
-      (forall ext : ByteString, decode_unused_word' sz (mappend b ext) = Some ((), mappend b' ext)).
-Proof.
-Admitted.
-
-Lemma computes_to_compose_decode_word
-     : forall (sz : nat) (w : word sz) (ctx ctx'' : CacheFormat)
-         (rest : CacheFormat -> Comp (ByteString * CacheFormat))
-         (b : ByteString),
-       (format_word w ThenC rest) ctx ↝ (b, ctx'') ->
-       exists (b' : ByteString) (ctx' : CacheFormat),
-         rest ctx' ↝ (b', ctx'') /\
-         (forall ext : ByteString, decode_word' sz (mappend b ext) = Some (w, mappend b' ext)).
-Proof.
-Admitted.
-
-Lemma IPv4_Packet_Header_Len_OK
-  : forall ip4 (ctx ctx' ctx'' : CacheFormat) c b b'' ext,
-    (format_word (natToWord 4 4)
-    ThenC format_nat 4 (IPv4_Packet_Header_Len ip4)
-    ThenC format_unused_word 8 (* TOS Field! *)
-    ThenC format_word ip4!"TotalLength"
-    ThenC format_word ip4!"ID"
-    ThenC format_unused_word 1 (* Unused flag! *)
-    ThenC format_bool ip4!"DF"
-    ThenC format_bool ip4!"MF"
-    ThenC format_word ip4!"FragmentOffset"
-    ThenC format_word ip4!"TTL"
-    ThenC format_enum ProtocolTypeCodes ip4!"Protocol"
-    DoneC) ctx ↝ (b, ctx') ->
-    (format_word ip4!"SourceAddress"
-    ThenC format_word ip4!"DestAddress"
-    ThenC format_list format_word ip4!"Options"
-    DoneC) ctx' ↝ (b'', ctx'') ->
-    IPv4_Packet_OK ip4 ->
-    (fun _ => 128) ip4 + (fun a => 16 + |ip4!"Options"| * 32) ip4 + (bin_measure mempty) + 16 = IPv4_Packet_formatd_measure (mappend (mappend b (mappend (format_checksum _ _ _ 16 c) b'')) ext).
-Proof.
-  intros.
-  set (k := mempty); simpl in k; subst k.
-  simpl bin_measure.
-  rewrite AlignedByteString.length_ByteString_id.
-  unfold IPv4_Packet_formatd_measure.
-  pose proof mappend_assoc as H'; simpl in H';
-    rewrite <- !H'.
-  eapply computes_to_compose_decode_unused_word in H;
-    let H' := fresh in
-    destruct H as [? [? [? H'] ] ]; rewrite H'.
-  unfold DecodeBindOpt, BindOpt, If_Opt_Then_Else.
-  eapply computes_to_compose_decode_word in H;
-    let H' := fresh in
-    destruct H as [? [? [? H'] ] ]; rewrite H'.
-  unfold fst.
-  rewrite wordToNat_natToWord_idempotent; try reflexivity;
-    eauto using IPv4_Packet_Headiner_Len_Bound.
-  unfold IPv4_Packet_Header_Len.
-  rewrite Mult.mult_plus_distr_l.
-  omega.
-Qed.
-
 Hint Resolve IPv4_Packet_Header_Len_eq : data_inv_hints.
 
-(* A (hopefully) more convenient IP_Checksum lemma *)
-
-Definition decode_IPChecksum
-  : ByteString -> CacheDecode -> option (() * ByteString * CacheDecode) :=
-  decode_unused_word 16.
-
-Definition encode_word {sz} (w : word sz) : ByteString :=
-  encode_word' sz w ByteString_id.
-
-Definition IPChecksum (b b' : ByteString) : ByteString :=
-  let b'' := if Peano_dec.eq_nat_dec (padding b) 0 then mempty
-             else encode_word (wzero (8 - (padding b))) in
-  mappend b''
-            (encode_word (wnot (onesComplement
-                                  (ByteString2ListOfChar (bin_measure (mappend b b')) (BoundedByteStringToByteString(mappend b b')))))).
-
-Definition IPChecksum_Valid_dec (n : nat) (b : ByteString)
-  : {IPChecksum_Valid' n b} + {~IPChecksum_Valid' n b} := weq _ _.
-
-Lemma CorrectAlignedDecoderForIPChecksumThenC {A}
-      predicate
-      (format_A format_B : FormatM A ByteString)
-      (len_format_A : A -> nat)
-      (len_format_A_OK : forall a' b ctx ctx',
-          computes_to (format_A a' ctx) (b, ctx')
-          -> length_ByteString b = len_format_A a')
-  : CorrectAlignedDecoderFor
-      predicate
-      (fun a => (format_A a) ThenC format_unused_word 16 ThenC (format_B a))
-    -> CorrectAlignedDecoderFor
-      predicate
-      (fun a => (format_A a) ThenChecksum IPChecksum_Valid' OfSize 16 ThenCarryOn (format_B a)).
-  Proof.
-    intros H; destruct H as [ ? [ [? ?] ?] ].
-  Admitted.
-
-Lemma length_ByteString_compose :
-  forall format1 format2 b (ctx ctx' : CacheFormat) n n',
-    computes_to (compose _ format1 format2 ctx) (b, ctx')
-    -> (forall ctx b ctx', computes_to (format1 ctx) (b, ctx')
-                           -> length_ByteString b = n)
-    -> (forall ctx b ctx', computes_to (format2 ctx) (b, ctx')
-                           -> length_ByteString b = n')
-    -> length_ByteString b = n + n'.
-Proof.
-  unfold compose, Bind2; intros; computes_to_inv; injections.
-  destruct v; destruct v0.
-  rewrite length_ByteString_enqueue_ByteString; erewrite H0, H1; eauto.
-Qed.
-
-Lemma length_ByteString_composeChecksum :
-  forall sz checksum_Valid format1 format2 b (ctx ctx' : CacheFormat) n n' ,
-    computes_to (composeChecksum _ _ _ sz checksum_Valid format1 format2 ctx) (b, ctx')
-    -> (forall ctx b ctx', computes_to (format1 ctx) (b, ctx')
-                           -> length_ByteString b = n)
-    -> (forall ctx b ctx', computes_to (format2 ctx) (b, ctx')
-                           -> length_ByteString b = n')
-    -> length_ByteString b = n + n' + sz.
-Proof.
-  unfold composeChecksum, Bind2; intros; computes_to_inv; injections.
-  destruct v; destruct v0.
-  rewrite !length_ByteString_enqueue_ByteString; simpl.
-  unfold format_checksum.
-  erewrite AlignedAutomation.length_encode_word'; simpl; rewrite AlignedByteString.length_ByteString_id.
-  erewrite H0, H1; eauto; omega.
-Qed.
-
-Lemma length_ByteString_composeIf :
-  forall format1 format2 b (ctx ctx' : CacheFormat) n P,
-    computes_to (composeIf _ _ _ P format1 format2 ctx) (b, ctx')
-    -> (forall ctx b ctx', computes_to (format1 ctx) (b, ctx')
-                           -> length_ByteString b = n)
-    -> (forall ctx b ctx', computes_to (format2 ctx) (b, ctx')
-                           -> length_ByteString b = n)
-    -> length_ByteString b = n.
-Proof.
-  unfold composeIf, Bind2; intros; computes_to_inv; injections.
-  destruct v; simpl in *; eauto.
-Qed.
-
-Lemma length_ByteString_ret :
-  forall b' b (ctx ctx' : CacheFormat),
-    computes_to (ret (b', ctx)) (b, ctx')
-    -> length_ByteString b = length_ByteString b'.
-Proof.
-  intros; computes_to_inv; injections; reflexivity.
-Qed.
-
-Lemma length_ByteString_unused_word
-  : forall sz (b : ByteString) (ctx ctx' : CacheFormat),
-    format_unused_word sz ctx ↝ (b, ctx')
-    -> length_ByteString b = sz.
-Proof.
-  unfold format_unused_word, format_unused_word'; simpl.
-  intros; computes_to_inv; injections.
-  rewrite AlignedAutomation.length_encode_word'; simpl.
-  rewrite AlignedByteString.length_ByteString_id.
-  omega.
-Qed.
-
-Lemma length_ByteString_word
-  : forall sz (w : word sz) (b : ByteString) (ctx ctx' : CacheFormat),
-    WordOpt.format_word w ctx ↝ (b, ctx')
-    -> length_ByteString b = sz.
-Proof.
-  unfold WordOpt.format_word; simpl.
-  intros; computes_to_inv; injections.
-  rewrite AlignedAutomation.length_encode_word'.
-  simpl; rewrite AlignedByteString.length_ByteString_id; omega.
-Qed.
-
-Lemma length_ByteString_bool
-  : forall (b' : bool) (b : ByteString) (ctx ctx' : CacheFormat),
-    format_bool b' ctx ↝ (b, ctx')
-    -> length_ByteString b = 1.
-Proof.
-  intros; eapply AlignedAutomation.length_ByteString_bool; eauto.
-Qed.
-
-Lemma length_ByteString_format_list {A}
-  : forall format_A l (b : ByteString) (ctx ctx' : CacheFormat) n,
-    (forall (a : A) (b : ByteString) (ctx ctx' : CacheFormat),
-        computes_to (format_A a ctx) (b, ctx')
-        -> length_ByteString b = n)
-    -> format_list format_A l ctx ↝ (b, ctx')
-    -> length_ByteString b = (length l) * n.
-Proof.
-  induction l; simpl; intros; computes_to_inv.
-  - injections; reflexivity.
-  - unfold Bind2 in H0; computes_to_inv; injections.
-    destruct v; destruct v0; simpl in *.
-    erewrite length_ByteString_enqueue_ByteString.
-    erewrite H; eauto.
-    rewrite Mult.mult_succ_l.
-    erewrite <- IHl; eauto with arith.
-Qed.
-
-Lemma ByteString_enqueue_padding_eq
-  : forall a b,
-    padding (ByteString_enqueue a b) =
-    NPeano.modulo (S (padding b)) 8.
-Proof.
-  intros.
-Admitted.
-
-Lemma queue_into_ByteString_padding_eq
-  : forall l,
-    padding (queue_into_ByteString l) = NPeano.modulo (length l) 8.
-Proof.
-Admitted.
-
-Lemma ByteString_enqueue_ByteString_padding_eq
-  : forall b b',
-    padding (ByteString_enqueue_ByteString b b') = NPeano.modulo (padding b + padding b') 8.
-Proof.
-  Admitted.
-
-Definition length_ByteString_ByteString_id
-  : length_ByteString ByteString_id = 0 := eq_refl.
-
-Lemma length_ByteString_format_option {A}
-  : forall format_Some format_None a_opt
-           (b : ByteString) (ctx ctx' : CacheFormat) n,
-    (forall (a : A) (b : ByteString) (ctx ctx' : CacheFormat),
-        computes_to (format_Some a ctx) (b, ctx')
-        -> length_ByteString b = n)
-    -> (forall (b : ByteString) (ctx ctx' : CacheFormat),
-           computes_to (format_None () ctx) (b, ctx')
-           -> length_ByteString b = n)
-    -> Option.format_option format_Some format_None a_opt ctx ↝ (b, ctx')
-    -> length_ByteString b = n.
-Proof.
-  destruct a_opt; simpl; intros; computes_to_inv.
-  - eapply H; eauto.
-  - eauto.
-Qed.
-
-Ltac calculate_length_ByteString :=
-  intros;
-   match goal with
-   | H:_ ↝ _
-     |- _ =>
-         (first
-          [ eapply (length_ByteString_composeChecksum _ _ _ _ _ _ _ _ _ H);
-             try (simpl mempty; rewrite length_ByteString_ByteString_id)
-          | eapply (length_ByteString_composeIf _ _ _ _ _ _ _ H);
-             try (simpl mempty; rewrite length_ByteString_ByteString_id)
-          | eapply (length_ByteString_compose _ _ _ _ _ _ _ H);
-             try (simpl mempty; rewrite length_ByteString_ByteString_id)
-          | eapply (fun H' H'' => length_ByteString_format_option _ _ _ _ _ _ _ H' H'' H)
-          | eapply (length_ByteString_unused_word _ _ _ _ H)
-          | eapply (length_ByteString_bool _ _ _ _ H)
-          | eapply (length_ByteString_word _ _ _ _ _ H)
-          | eapply (fun H' => length_ByteString_format_list _ _ _ _ _ _ H' H)
-          | eapply (length_ByteString_ret _ _ _ _ H) ]);
-          clear H
-   end.
-
-
-  Lemma AlignedDecode_Throw {A}
-    : DecodeMEquivAlignedDecodeM (fun (_ : ByteString) (_ : CacheDecode) => None)
-                                 (fun sz : nat => ThrowAlignedDecodeM (A := A)).
-  Proof.
-    unfold DecodeMEquivAlignedDecodeM; intuition; try discriminate.
-  Qed.
-  
-  Lemma AlignedDecode_ifb {A : Type}
-        (decode_A : DecodeM A ByteString)
-        (cond : bool)
-        (aligned_decoder : forall numBytes : nat, AlignedDecodeM A numBytes)
-    : DecodeMEquivAlignedDecodeM
-        decode_A
-        aligned_decoder
-      -> DecodeMEquivAlignedDecodeM
-        (fun bs cd => if cond
-                      then decode_A bs cd
-                      else None)
-        (fun sz => if cond
-                   then aligned_decoder sz
-                   else ThrowAlignedDecodeM).
-  Proof.
-    intros; destruct cond; simpl; eauto using AlignedDecode_Throw.
-  Qed.
-
-  Lemma AlignedDecode_Sumb {A : Type}
-        (decode_A : DecodeM A ByteString)
-        (P : Prop)
-        (cond : {P} + {~P})
-        (aligned_decoder : forall numBytes : nat, AlignedDecodeM A numBytes)
-    : DecodeMEquivAlignedDecodeM
-        decode_A
-        aligned_decoder
-      -> DecodeMEquivAlignedDecodeM
-        (fun bs cd => if cond
-                      then decode_A bs cd
-                      else None)
-        (fun sz => if cond
-                   then aligned_decoder sz
-                   else ThrowAlignedDecodeM).
-  Proof.
-    intros; destruct cond; simpl; eauto using AlignedDecode_Throw.
-  Qed.
-
-  Definition SkipCurrentByte (* Gets the current byte and increments the current index. *)
-             {n : nat}
-    : AlignedDecodeM () n :=
-    fun v idx c => Ifopt (nth_opt v idx) as b Then Some ((), S idx, addD c 8) Else None.
-
-  Lemma AlignedDecodeUnusedCharM
-    : DecodeMEquivAlignedDecodeM
-           (decode_unused_word (monoidUnit := ByteString_QueueMonoidOpt) 8)
-           (fun numBytes => SkipCurrentByte).
-  Proof.
-    unfold DecodeMEquivAlignedDecodeM, BindAlignedDecodeM, DecodeBindOpt2, BindOpt; intros;
-      unfold decode_unused_word, decode_unused_word'.
-    split; [ | split ]; intros.
-    - pattern numBytes_hd, v; eapply Vector.caseS; simpl; intros.
-      unfold SkipCurrentByte; simpl.
-      destruct (nth_opt t n); simpl; eauto.
-  Admitted.
-
-  Lemma AlignedDecodeBindCharM' {A C : Type}
-        (t : word 8 -> DecodeM C ByteString)
-        (t' : word 8 -> forall {numBytes}, AlignedDecodeM C numBytes)
-        decode_w
-    : (forall v cd,
-          decode_word (monoidUnit := ByteString_QueueMonoidOpt) (sz := 8) v cd
-          = decode_w v cd)
-      -> (forall b, DecodeMEquivAlignedDecodeM (t b) (@t' b))        
-      -> DecodeMEquivAlignedDecodeM
-           (fun v cd => `(a, b0, cd') <- decode_w v cd;
-                          t a b0 cd')
-           (fun numBytes => b <- GetCurrentByte; t' b)%AlignedDecodeM.
-  Proof.
-    intros; eapply Bind_DecodeMEquivAlignedDecodeM; eauto.
-    eapply DecodeMEquivAlignedDecodeM_trans; eauto.
-    apply AlignedDecodeCharM.
-    simpl. intros; eapply AlignedDecodeMEquiv_refl.
-  Qed.
-
-
-  Lemma AlignedDecode_assoc {A B C : Type}
-        (decode_A : DecodeM A ByteString)
-        (decode_B : A -> DecodeM B ByteString)
-        (decode_C : A -> B -> DecodeM C ByteString)
-        (aligned_decoder : forall numBytes : nat, AlignedDecodeM C numBytes)
-    : DecodeMEquivAlignedDecodeM
-        (fun bs cd => `(ab, bs', cd') <- (`(a, bs', cd') <- decode_A bs cd;
-                                            `(b, bs', cd') <- decode_B a bs' cd';
-                                            Some (a, b, bs', cd'));
-                      decode_C (fst ab) (snd ab) bs' cd')
-        aligned_decoder
-      -> DecodeMEquivAlignedDecodeM
-           (fun bs cd => `(a, bs', cd') <- decode_A bs cd;
-                           `(b, bs', cd') <- decode_B a bs' cd';
-                           decode_C a b bs' cd')
-           aligned_decoder.
-  Proof.
-    intros; eapply DecodeMEquivAlignedDecodeM_trans; eauto;
-      intros; simpl; try reflexivity.
-    simpl; destruct (decode_A b cd) as [ [ [? ?] ?] | ]; simpl; eauto.
-    destruct (decode_B a b0 c) as [ [ [? ?] ?] | ]; simpl; eauto.
-  Qed.
-  
-  Lemma AlignedDecodeBindUnusedCharM {C : Type}
-        (t : unit -> DecodeM C ByteString)
-        (t' : unit -> forall {numBytes}, AlignedDecodeM C numBytes)
-    : (DecodeMEquivAlignedDecodeM (t ()) (@t' ()))
-      -> DecodeMEquivAlignedDecodeM
-           (fun v cd => `(a, b0, cd') <- decode_unused_word (monoidUnit := ByteString_QueueMonoidOpt) 8 v cd;
-                          t a b0 cd')
-           (fun numBytes => b <- SkipCurrentByte; @t' b numBytes)%AlignedDecodeM.
-  Proof.
-    intro; eapply Bind_DecodeMEquivAlignedDecodeM; eauto using AlignedDecodeUnusedCharM.
-    intro; destruct a; eauto.
-  Qed.
-  Arguments wordToNat : simpl never.  
+Arguments wordToNat : simpl never.
 
 Definition EthernetHeader_decoder
   : CorrectAlignedDecoderFor IPv4_Packet_OK IPv4_Packet_Format.
 Proof.
-
-  unfold IPv4_Packet_Format.
   eapply CorrectAlignedDecoderForIPChecksumThenC.
   cbv beta; unfold Domain; simpl; repeat calculate_length_ByteString.
   unfold IPv4_Packet_OK.
-  Arguments plus : simpl never.
   start_synthesizing_decoder.
   normalize_compose AlignedByteString.ByteStringQueueMonoid.
   decode_step idtac.
@@ -532,71 +124,83 @@ Proof.
   eapply @AlignedDecoders.AlignedDecode_Sumb.
   eapply @AlignedDecode_CollapseWord; eauto.
   eapply @AlignedDecodeBindCharM; intros.
-  intros; apply @AlignedDecode_Sumb.  
-  eapply @AlignedDecodeBindUnusedCharM; simpl.
-  eapply DecodeMEquivAlignedDecodeM_trans.
-  2: intros; reflexivity.
+  intros; apply @AlignedDecode_Sumb.
+  eapply @AlignedDecodeBindUnusedCharM; simpl;
+    eapply DecodeMEquivAlignedDecodeM_trans;
+      [ | intros; reflexivity
+        |  ].
   eapply @AlignedDecodeBind2CharM; intros; eauto.
   eapply @AlignedDecodeBind2CharM; intros; eauto.
   eapply @AlignedDecoders.AlignedDecode_Sumb.
-  eapply AlignedDecode_assoc.
+  eapply AlignedDecode_CollapseWord';
+    eauto using decode_word_eq_decode_unused_word,
+    decode_word_eq_decode_bool,
+    decode_word_eq_decode_word.
   eapply @AlignedDecoders.AlignedDecode_Sumb.
-  eapply AlignedDecode_assoc.
+  eapply AlignedDecode_CollapseWord';
+    eauto using decode_word_eq_decode_unused_word,
+    decode_word_eq_decode_bool,
+    decode_word_eq_decode_word.
   eapply @AlignedDecoders.AlignedDecode_Sumb.
-  eapply AlignedDecode_assoc.
-  eapply @AlignedDecoders.AlignedDecode_Sumb.
-  
-  
-  setoid_rewrite <- @DecodeBindOpt2_assoc.
-  Locate "`(".
-  
-  
-  
-  
-
-  unfold monoid.
-  eauto.
-
-  cbv beta; align_decoders.
-
+  eapply AlignedDecode_CollapseWord';
+    eauto using decode_word_eq_decode_unused_word,
+    decode_word_eq_decode_bool,
+    decode_word_eq_decode_word.
+  eapply @AlignedDecodeBind2CharM; intros; eauto.
+  eapply @AlignedDecodeBindCharM; intros; eauto.
+  eapply @AlignedDecodeBindEnumM; intros; eauto.
+  eapply @AlignedDecodeBindUnused2CharM; simpl;
+    eapply DecodeMEquivAlignedDecodeM_trans;
+      [ | intros; reflexivity
+        |  ].
+  eapply @AlignedDecodeBind4CharM; intros; eauto.
+  eapply @AlignedDecodeBind4CharM; intros; eauto.
+  eapply @AlignedDecodeListM; intros; eauto.
+  eapply (fun H H' => @AlignedDecodeNCharM _ _ H H' 4); eauto; simpl; intros.
+  eapply @AlignedDecode_ifb.
+  eapply @Return_DecodeMEquivAlignedDecodeM.
+  intros; higher_order_reflexivity.
+  intros; higher_order_reflexivity.
 Defined.
 
-Definition IPv4_decoder_impl :=
-  Eval simpl in (fst (proj1_sig EthernetHeader_decoder)).
+Definition IPv4_decoder_impl {sz} v :=
+  Eval simpl in (projT1 EthernetHeader_decoder sz v 0 ()).
 
-Definition pkt' : list char :=
+Definition pkt' : Vector.t (word 8) _ :=
   [WO~1~0~1~0~0~0~1~0;
-   WO~0~0~0~0~0~0~0~0;
+     WO~0~0~0~0~0~0~0~0;
 
-   WO~0~0~0~0~0~0~0~0;
-   WO~0~0~0~0~0~0~0~0;
+     WO~0~0~0~0~0~0~0~0;
+     WO~0~0~0~0~0~0~0~0;
 
-   WO~0~0~0~0~0~0~0~0;
-   WO~0~0~0~0~0~0~0~0;
+     WO~0~0~0~0~0~0~0~0;
+     WO~0~0~0~0~0~0~0~0;
 
-   WO~0~0~0~0~0~0~0~0;
-   WO~0~0~0~0~0~0~0~0;
+     WO~0~0~0~0~0~0~0~0;
+     WO~0~0~0~0~0~0~0~0;
 
-   WO~0~1~1~0~0~1~0~0;
-   WO~1~0~0~0~0~0~0~0;
+     WO~0~1~1~0~0~1~0~0;
+     WO~1~0~0~0~0~0~0~0;
 
-   WO~0~0~0~0~0~0~0~0;
-   WO~0~0~0~0~0~0~0~0;
+     WO~0~0~0~0~0~0~0~0;
+     WO~0~0~0~0~0~0~0~0;
 
-   WO~0~0~0~0~0~0~1~1;
-   WO~0~0~0~1~0~1~0~1;
+     WO~0~0~0~0~0~0~1~1;
+     WO~0~0~0~1~0~1~0~1;
 
-   WO~0~1~1~1~1~0~1~1;
-   WO~0~1~0~1~0~0~0~0;
+     WO~0~1~1~1~1~0~1~1;
+     WO~0~1~0~1~0~0~0~0;
 
-   WO~0~0~0~0~0~0~1~1;
-   WO~0~0~0~1~0~1~0~1;
+     WO~0~0~0~0~0~0~1~1;
+     WO~0~0~0~1~0~1~0~1;
 
-   WO~0~1~1~1~1~0~1~1;
-   WO~1~0~0~0~0~0~0~0]%list.
+     WO~0~1~1~1~1~0~1~1;
+     WO~1~0~0~0~0~0~0~0].
 
-Definition pkt : list char :=
-    Eval compute in map (@natToWord 8) [69;0;100;0;0;0;0;0;38;1;243;159;192;168;222;10;192;168;222;1;0;0;0;0].
+Definition pkt : Vector.t (word 8) _ :=
+  Eval compute in Vector.map (@natToWord 8) [69;0;100;0;0;0;0;0;38;1;243;159;192;168;222;10;192;168;222;1;0;0;0;0].
+
+Eval vm_compute in (IPv4_decoder_impl _ pkt 0 ()).
 
 Compute (InternetChecksum.checksum pkt).
 
