src/Narcissus/BinLib/AlignedIPChecksum.v
@@ -1,0 +1,228 @@
+Require Import
+        Coq.Strings.String
+        Coq.Vectors.Vector
+        Coq.omega.Omega.
+
+Require Import
+        Fiat.Common.SumType
+        Fiat.Common.EnumType
+        Fiat.Common.BoundedLookup
+        Fiat.Common.ilist
+        Fiat.Computation
+        Fiat.QueryStructure.Specification.Representation.Notations
+        Fiat.QueryStructure.Specification.Representation.Heading
+        Fiat.QueryStructure.Specification.Representation.Tuple
+        Fiat.Narcissus.BinLib.AlignedByteString
+        Fiat.Narcissus.BinLib.AlignWord
+        Fiat.Narcissus.BinLib.AlignedList
+        Fiat.Narcissus.BinLib.AlignedDecoders
+        Fiat.Narcissus.BinLib.AlignedDecodeMonad
+        Fiat.Narcissus.BinLib.AlignedEncodeMonad
+        Fiat.Narcissus.Common.Specs
+        Fiat.Narcissus.Common.WordFacts
+        Fiat.Narcissus.Common.ComposeCheckSum
+        Fiat.Narcissus.Common.ComposeIf
+        Fiat.Narcissus.Common.ComposeOpt
+        Fiat.Narcissus.Automation.Solver
+        Fiat.Narcissus.Automation.AlignedAutomation
+        Fiat.Narcissus.Formats
+        Fiat.Narcissus.Stores.EmptyStore.
+
+Require Import Bedrock.Word.
+
+Definition decode_IPChecksum
+  : ByteString -> CacheDecode -> option (() * ByteString * CacheDecode) :=
+  decode_unused_word 16.
+
+Definition encode_word {sz} (w : word sz) : ByteString :=
+  encode_word' sz w ByteString_id.
+
+Definition IPChecksum (b b' : ByteString) : ByteString :=
+  let b'' := if Peano_dec.eq_nat_dec (padding b) 0 then mempty
+             else encode_word (wzero (8 - (padding b))) in
+  mappend b''
+          (encode_word (wnot (onesComplement
+                                (ByteString2ListOfChar (bin_measure (mappend b b')) (BoundedByteStringToByteString(mappend b b')))))).
+
+Definition IPChecksum_Valid_dec (n : nat) (b : ByteString)
+  : {IPChecksum_Valid' n b} + {~IPChecksum_Valid' n b} := weq _ _.
+
+Lemma CorrectAlignedDecoderForIPChecksumThenC {A}
+      predicate
+      (format_A format_B : FormatM A ByteString)
+      (len_format_A : A -> nat)
+      (len_format_A_OK : forall a' b ctx ctx',
+          computes_to (format_A a' ctx) (b, ctx')
+          -> length_ByteString b = len_format_A a')
+  : CorrectAlignedDecoderFor
+      predicate
+      (fun a => (format_A a) ThenC format_unused_word 16 ThenC (format_B a))
+    -> CorrectAlignedDecoderFor
+         predicate
+         (fun a => (format_A a) ThenChecksum IPChecksum_Valid' OfSize 16 ThenCarryOn (format_B a)).
+Proof.
+  intros H; destruct H as [ ? [ [? ?] ?] ].
+  eexists _, (_, _).
+Admitted.
+
+Lemma length_ByteString_compose :
+  forall format1 format2 b (ctx ctx' : CacheFormat) n n',
+    computes_to (compose _ format1 format2 ctx) (b, ctx')
+    -> (forall ctx b ctx', computes_to (format1 ctx) (b, ctx')
+                           -> length_ByteString b = n)
+    -> (forall ctx b ctx', computes_to (format2 ctx) (b, ctx')
+                           -> length_ByteString b = n')
+    -> length_ByteString b = n + n'.
+Proof.
+  unfold compose, Bind2; intros; computes_to_inv; injections.
+  destruct v; destruct v0.
+  rewrite length_ByteString_enqueue_ByteString; erewrite H0, H1; eauto.
+Qed.
+
+Lemma length_ByteString_composeChecksum :
+  forall sz checksum_Valid format1 format2 b (ctx ctx' : CacheFormat) n n' ,
+    computes_to (composeChecksum _ _ _ sz checksum_Valid format1 format2 ctx) (b, ctx')
+    -> (forall ctx b ctx', computes_to (format1 ctx) (b, ctx')
+                           -> length_ByteString b = n)
+    -> (forall ctx b ctx', computes_to (format2 ctx) (b, ctx')
+                           -> length_ByteString b = n')
+    -> length_ByteString b = n + n' + sz.
+Proof.
+  unfold composeChecksum, Bind2; intros; computes_to_inv; injections.
+  destruct v; destruct v0.
+  rewrite !length_ByteString_enqueue_ByteString; simpl.
+  unfold format_checksum.
+  erewrite AlignedAutomation.length_encode_word'; simpl; rewrite AlignedByteString.length_ByteString_id.
+  erewrite H0, H1; eauto; omega.
+Qed.
+
+Lemma length_ByteString_composeIf :
+  forall format1 format2 b (ctx ctx' : CacheFormat) n P,
+    computes_to (composeIf _ _ _ P format1 format2 ctx) (b, ctx')
+    -> (forall ctx b ctx', computes_to (format1 ctx) (b, ctx')
+                           -> length_ByteString b = n)
+    -> (forall ctx b ctx', computes_to (format2 ctx) (b, ctx')
+                           -> length_ByteString b = n)
+    -> length_ByteString b = n.
+Proof.
+  unfold composeIf, Bind2; intros; computes_to_inv; injections.
+  destruct v; simpl in *; eauto.
+Qed.
+
+Lemma length_ByteString_ret :
+  forall b' b (ctx ctx' : CacheFormat),
+    computes_to (ret (b', ctx)) (b, ctx')
+    -> length_ByteString b = length_ByteString b'.
+Proof.
+  intros; computes_to_inv; injections; reflexivity.
+Qed.
+
+Lemma length_ByteString_unused_word
+  : forall sz (b : ByteString) (ctx ctx' : CacheFormat),
+    format_unused_word sz ctx ↝ (b, ctx')
+    -> length_ByteString b = sz.
+Proof.
+  unfold format_unused_word, format_unused_word'; simpl.
+  intros; computes_to_inv; injections.
+  rewrite AlignedAutomation.length_encode_word'; simpl.
+  rewrite AlignedByteString.length_ByteString_id.
+  omega.
+Qed.
+
+Lemma length_ByteString_word
+  : forall sz (w : word sz) (b : ByteString) (ctx ctx' : CacheFormat),
+    WordOpt.format_word w ctx ↝ (b, ctx')
+    -> length_ByteString b = sz.
+Proof.
+  unfold WordOpt.format_word; simpl.
+  intros; computes_to_inv; injections.
+  rewrite AlignedAutomation.length_encode_word'.
+  simpl; rewrite AlignedByteString.length_ByteString_id; omega.
+Qed.
+
+Lemma length_ByteString_bool
+  : forall (b' : bool) (b : ByteString) (ctx ctx' : CacheFormat),
+    format_bool b' ctx ↝ (b, ctx')
+    -> length_ByteString b = 1.
+Proof.
+  intros; eapply AlignedAutomation.length_ByteString_bool; eauto.
+Qed.
+
+Lemma length_ByteString_format_list {A}
+  : forall format_A l (b : ByteString) (ctx ctx' : CacheFormat) n,
+    (forall (a : A) (b : ByteString) (ctx ctx' : CacheFormat),
+        computes_to (format_A a ctx) (b, ctx')
+        -> length_ByteString b = n)
+    -> format_list format_A l ctx ↝ (b, ctx')
+    -> length_ByteString b = (length l) * n.
+Proof.
+  induction l; simpl; intros; computes_to_inv.
+  - injections; reflexivity.
+  - unfold Bind2 in H0; computes_to_inv; injections.
+    destruct v; destruct v0; simpl in *.
+    erewrite length_ByteString_enqueue_ByteString.
+    erewrite H; eauto.
+    rewrite Mult.mult_succ_l.
+    erewrite <- IHl; eauto with arith.
+Qed.
+
+Lemma ByteString_enqueue_padding_eq
+  : forall a b,
+    padding (ByteString_enqueue a b) =
+    NPeano.modulo (S (padding b)) 8.
+Proof.
+  intros.
+Admitted.
+
+Lemma queue_into_ByteString_padding_eq
+  : forall l,
+    padding (queue_into_ByteString l) = NPeano.modulo (length l) 8.
+Proof.
+Admitted.
+
+Lemma ByteString_enqueue_ByteString_padding_eq
+  : forall b b',
+    padding (ByteString_enqueue_ByteString b b') = NPeano.modulo (padding b + padding b') 8.
+Proof.
+Admitted.
+
+Definition length_ByteString_ByteString_id
+  : length_ByteString ByteString_id = 0 := eq_refl.
+
+Lemma length_ByteString_format_option {A}
+  : forall format_Some format_None a_opt
+           (b : ByteString) (ctx ctx' : CacheFormat) n,
+    (forall (a : A) (b : ByteString) (ctx ctx' : CacheFormat),
+        computes_to (format_Some a ctx) (b, ctx')
+        -> length_ByteString b = n)
+    -> (forall (b : ByteString) (ctx ctx' : CacheFormat),
+           computes_to (format_None () ctx) (b, ctx')
+           -> length_ByteString b = n)
+    -> Option.format_option format_Some format_None a_opt ctx ↝ (b, ctx')
+    -> length_ByteString b = n.
+Proof.
+  destruct a_opt; simpl; intros; computes_to_inv.
+  - eapply H; eauto.
+  - eauto.
+Qed.
+
+Ltac calculate_length_ByteString :=
+  intros;
+  match goal with
+  | H:_ ↝ _
+    |- _ =>
+    (first
+       [ eapply (length_ByteString_composeChecksum _ _ _ _ _ _ _ _ _ H);
+         try (simpl mempty; rewrite length_ByteString_ByteString_id)
+       | eapply (length_ByteString_composeIf _ _ _ _ _ _ _ H);
+         try (simpl mempty; rewrite length_ByteString_ByteString_id)
+       | eapply (length_ByteString_compose _ _ _ _ _ _ _ H);
+         try (simpl mempty; rewrite length_ByteString_ByteString_id)
+       | eapply (fun H' H'' => length_ByteString_format_option _ _ _ _ _ _ _ H' H'' H)
+       | eapply (length_ByteString_unused_word _ _ _ _ H)
+       | eapply (length_ByteString_bool _ _ _ _ H)
+       | eapply (length_ByteString_word _ _ _ _ _ H)
+       | eapply (fun H' => length_ByteString_format_list _ _ _ _ _ _ H' H)
+       | eapply (length_ByteString_ret _ _ _ _ H) ]);
+    clear H
+  end.
